theories/AlmostStlc/Compatibility.v
@@ -16,11 +16,14 @@ Local Open Scope monad_scope.
 Require Export SemanticsFactsSeq.
 Require Export CallMrecFacts.
 Require Export SemanticsFactsSeq2.
+Require Export SmallStepSeqFacts.
 Require Import Lia.
 Require Import Coq.Classes.Morphisms.
 Require Export ClosingSubst.
 Require Export LogicalApprox.
 Require Export RecursionTrace.
+Require Export ApproxCompTerm.
+From Paco Require Import paco.
 
 Definition denote_comp_type t Γ MR : Type :=
   denote_ctx Γ -> mtree (denote_mfix_ctx MR) (denote_type t).
@@ -75,14 +78,13 @@ Proof.
     rewrite Heqx. auto.
 Qed.
 
-(*
-(* this might need to be an inductive proof *)
-Lemma let_compat Γ MR t1 t2 
-      (m1 : denote_comp_type t1 Γ MR) (m2 : denote_comp_type t2 (t1 :: Γ) MR)
-      (c1 : comp t1 Γ MR) (c2 : comp t2 (t1 :: Γ) MR)
-  : comp_rel m1 c1 -> comp_rel m2 c2 ->
-    comp_rel (comp_bind m1 m2) (comp_let c1 c2).
-*)
+Lemma weaken_r_value_nil_nil : forall t (v : value t []),
+    weaken_r_value [] v = v.
+Proof.
+  intros. unfold weaken_r_value. rewrite val_map_id; auto.
+  intros. inversion x.
+Qed.
+
 Lemma let_compat_aux n : forall Γ MR t1 t2
       (m1 : denote_comp_type t1 Γ MR) (m2 : denote_comp_type t2 (t1 :: Γ) MR)
       (c1 : comp t1 Γ MR) (c2 : comp t2 (t1 :: Γ) MR),
@@ -91,14 +93,12 @@ Lemma let_compat_aux n : forall Γ MR t1 t2
 Proof.
   induction n as [ n' IHn' ] using (well_founded_induction lt_wf).
   intros ? ? ? ? ? ? ? ? Hmc1 Hmc2 n hyps ρ Hn' Hhρ.
-  (* can I just make this inductive? *)
   constructor. intros j Hj. specialize (Hmc1 n hyps ρ Hn' Hhρ) as Hmc1n.
   inversion Hmc1n. subst. rename H into Happrox1.
   split.
   - intros vv2 Hvv2. unfold comp_bind in Hvv2.
     eapply multi_step_ret_bind_inv in Hvv2.
     destruct Hvv2 as [j1 [j2 [vv1 [Hn [Hvv11 Hvv12] ]]]].
-    (* problem here, look into it tomorrow, might be introducing *)
     assert (Hj1 : j1 < n). lia.
     specialize (Happrox1 j1 Hj1). destruct Happrox1 as [Hretmc1 _].
     specialize (Hretmc1 vv1 Hvv11).
@@ -113,7 +113,8 @@ Proof.
     specialize (H j2 Hj2). destruct H as [Hretmc2 _ ].
     specialize (Hretmc2 _ Hvv12). destruct Hretmc2 as [v2 [Hv21 Hv22]].
     exists v2. split.
-    + (* need stepping metatheory, can be a focus next week *) admit.
+    + rewrite close_comp_let. eapply eval_rel_stuck_let1; eauto.
+      rewrite subst_comp_const_close. eauto.
     + assert (n - j = n - j1 - j2). lia. rewrite H. auto.
   - intros. rename H into Hcall.
     eapply multi_step_call_term_bind_inv in Hcall.
@@ -135,32 +136,86 @@ Proof.
       split; [| split]; [| | split]; eauto.
       * assert (H : n - j1 - j2 = n - (j1 + j2)). lia. rewrite <- H.
         auto.
-      * admit. (* stepping metatheory *)
+      * rewrite close_comp_let. eapply eval_rel_stuck_let1; eauto.
+        rewrite subst_comp_const_close. auto.
       * intros. eapply HE3; eauto. lia.
     + specialize (Happrox1 j Hj). destruct Happrox1 as [_ Hstuckmc1].
       apply Hstuckmc1 in Hstep.
        destruct Hstep as [vcall [E [c' [Hvcall [HE1 [HE2 HE3 ]] ]]] ].
-       exists vcall. eexists. eexists. (* comp_let c' c2 with proper closing*) 
+       exists vcall. exists (ev_let E (close_comp_binder ρ c2) ). 
+       exists (comp_let c' (close_comp_binder ρ c2)). 
+       (* comp_let c' c2 with proper closing*) 
        split; [ | split]; [| | split]; eauto.
-       * admit. (* will require stepping metatheory *)
-       * admit. (* should be trivial once I can formalize the eval context 
-                  morally (ev_let E (close_comp Γ ρ c2)). but requires *)
+       * rewrite close_comp_let.
+         eapply eval_rel_stuck_let2; eauto.
+       * constructor. auto.
        * intros. rewrite <- Hk1'. clear Hstuckmc1.
          assert (Hj'' : j'' < n'). lia.
          specialize (IHn' j'' Hj'' [] MR t1 t2 (fun _ => k1' vvret) (fun '(vv2,_) => m2 (vv2, hyps))).
          specialize (IHn' (subst_eval_context E (comp_ret vret))).
-         unfold comp_bind in IHn'. admit.
-         (* the choice of c2 requires an open substitution thing, but should be fine*)
+         unfold comp_bind in IHn'. simp subst_eval_context. red in IHn'.
+         erewrite <- close_comp_equation_1. 
+         eapply IHn' with (hyps := tt) (ρ := tt).
+         -- red. intros j''' [] [] Hj''' _. simp close_comp. eapply HE3.
+            lia. inversion Hj'''. subst. auto. eapply lower_approx_val; try apply H0.
+            lia.
+         -- red. intros j''' [vv1 []] [v1 []] Hj''' Hvv1. 
+            dependent destruction Hvv1.
+            simp close_comp. rewrite <- close_comp_open. 
+            eapply Hmc2. lia. constructor. rewrite weaken_r_value_nil_nil. auto.
+            eapply lower_closing_subst_approx. eauto. lia.
+         -- lia.
+         -- constructor.
+Qed.
 
-         (* lots of details up in the air but this feels good *)
-         (* let Γ = [], m2 := fun vv2 => m2 (vv2, hyps), which I have knowledge about at j''*)
-         (* lets try to *)
-         (* I have info about k1' vvret at j'' or lower *)
-         (* I have infor about m2 at any level I have info about return of k1' vvret 
-            which is at most j'' *)
-         (* seems to fit with *)
- Admitted.
+Lemma let_approx n : forall MR t1 t2
+      (m1 : mtree (denote_mfix_ctx MR) (denote_type t1)) (k2 : denote_type t1 -> mtree (denote_mfix_ctx MR) (denote_type t2))
+      (c1 : comp t1 [] MR) (c2 : comp t2 [t1] MR),
+    approx_comp n approx_val m1 c1 -> 
+    (forall n0 vv1 v1, n0 <= n -> approx_val n0 t1 vv1 v1 -> approx_comp n0 approx_val (k2 vv1) (subst_comp_cons c2 v1)) ->
+    approx_comp n approx_val (bind m1 k2) (comp_let c1 c2).
+Proof.
+  intros. specialize let_compat_aux with (Γ := []) as Hlet. 
+  red in Hlet. specialize Hlet with (n := n) (j := n) (hyps := tt) (ρ := tt).
+  specialize (Hlet MR t1 t2 (fun _ => m1) (fun '(x, _) => k2 x) c1 c2).
+  unfold comp_bind in Hlet. simp close_comp in Hlet. apply Hlet; auto.
+  red. intros j [] [] Hj _. simp close_comp. eapply lower_approx_comp'; try apply H. lia. 
+  intros. eapply lower_approx_val; eauto.
+  red. intros j [vv1 []] [v1 []] Hj Happrox. dependent destruction Happrox. 2 : constructor.
+  simp close_comp. rewrite weaken_r_value_nil_nil. eapply H0; eauto.
+Qed.
 
+Lemma approx_comp_multi_step_minus:
+  forall (t : vtype) (R : call_frame) (MR : mfix_ctx) (c' : comp t [] (R :: MR)) 
+    (n : nat)
+    m1 m2
+    (n0 : nat),
+    n < n0 ->
+    approx_comp n0 approx_val m1 c' -> multi_step n m1 m2 -> approx_comp (n0 - n) approx_val m2 c'.
+Proof.
+  intros t R MR c' n m1 m2 n0.
+  intros Hnn0 Happrox Hstep. inversion Happrox. subst.
+  clear Happrox.
+  rename H into Happrox.
+  constructor. intros. split.
+  - assert (Hj' : j' + n < n0). lia.
+    specialize (Happrox _ Hj'). destruct Happrox as [Hret _].
+    intros vv Hstep'. 
+    assert (multi_step (n + j') m1 (ret vv)). eapply multi_step_add; eauto.
+    rewrite PeanoNat.Nat.add_comm in H0. specialize (Hret vv H0).
+    destruct Hret as [v [Hv1 Hv2]]. exists v.
+    split; auto. eapply lower_approx_val'; try apply Hv2. lia.
+ - assert (Hj' : j' + n < n0). lia.
+    specialize (Happrox _ Hj'). destruct Happrox as [_ Hstuck].
+    intros. 
+    assert (multi_step (n + j') m1 (vv <- call_term x xR vvcall;; k vv)).
+    eapply multi_step_add; eauto. rewrite PeanoNat.Nat.add_comm in H1.
+    specialize (Hstuck _ _ _ _ _ _ _ H1).
+    destruct Hstuck as [vcall [E [c'' [HE1 [HE2 [HE3 HE4]]]]]].
+    exists vcall, E, c''. split; [ | split; [ | split]]; auto.
+    eapply lower_approx_val'; try apply HE1. lia.
+    intros. eapply HE4; eauto. lia.
+Qed.
 
 Lemma let_compat Γ MR t1 t2 
       (m1 : denote_comp_type t1 Γ MR) (m2 : denote_comp_type t2 (t1 :: Γ) MR)
@@ -171,97 +226,530 @@ Proof.
   intros. red. intros. eapply let_compat_aux; try red; eauto.
 Qed.
 
+(* replace eq with beta equivalence  *)
+Lemma subst_eval_context__ctx n t1 MR1 t2 r (E : @eval_context t1 MR1 t2 MR1 r true) (c : comp t2 [] MR1) :
+  approx_comp_term n (subst_eval_context E c) (comp_let c (subst_eval_context_ctx E (comp_ret (val_var VarZ)))).
+Proof.
+  generalize dependent c. dependent induction E.
+  - intros. simp subst_eval_context. simp subst_eval_context_ctx. 
+    apply approx_comp_term_let_ret_r.
+  - intros c2. simp subst_eval_context. simp subst_eval_context_ctx. 
+    eapply approx_comp_term_trans. eapply approx_comp_term_let_cong. eauto. intros. apply approx_comp_term_refl.
+    eapply approx_comp_term_let_assoc.
+Qed.
+
+Lemma subst_eval_context__ctx' n t1 MR1 t2 r (E : @eval_context t1 MR1 t2 MR1 r true) (c : comp t2 [] MR1) :
+  approx_comp_term n (comp_let c (subst_eval_context_ctx E (comp_ret (val_var VarZ)))) (subst_eval_context E c).
+Proof.
+  generalize dependent c. dependent induction E.
+  - intros. simp subst_eval_context. simp subst_eval_context_ctx. 
+    apply approx_comp_term_let_ret_r'.
+  - intros c2. simp subst_eval_context. simp subst_eval_context_ctx. 
+    eapply approx_comp_term_trans. 2 : eapply approx_comp_term_let_cong; eauto.
+    2 : intros; try apply approx_comp_term_refl.
+    apply approx_comp_term_let_assoc'.
+Qed.
+
+
+(* TODO: this is currently unsound, relying on an equality when I need a seperate equivalence relation 
+   that is proper wrt approx_comp *)
+Lemma approx_comp_eval_context t1 MR1 t2 r (E : @eval_context t1 MR1 t2 MR1 r true)
+      (c : comp t2 [] MR1) m k n1 n2:
+  n1 < n2 ->
+         approx_comp n1 approx_val m c -> 
+  (forall n3 (vv2 : denote_type t2) (v2 : closed_value t2),
+      n3 < n2 -> approx_val n3 t2 vv2 v2 ->
+      approx_comp n3 approx_val (k vv2) (subst_eval_context E (comp_ret v2))) ->
+  approx_comp n1 approx_val (bind m k) (subst_eval_context E c).
+Proof.
+  intros Hn12 Hmc HkE. eapply approx_comp_approx_comp_term.
+  eapply subst_eval_context__ctx'.
+
+  (* might have done some of this in the wrong direction *)
+  eapply let_approx; eauto.
+  intros. eapply HkE in H0. 2 : lia.
+  enough ( (subst_comp_cons (SmallStepSeq.subst_eval_context_ctx E (comp_ret (val_var VarZ))) v1) 
+           = (subst_eval_context E (comp_ret v1))).
+  rewrite H1. auto.
+  clear. dependent induction E.
+  - simp subst_eval_context_ctx. unfold subst_comp_cons. simp subst_comp. simp subst_var.
+    simp subst_eval_context. auto.
+  - simp subst_eval_context_ctx. unfold subst_comp_cons. simp subst_comp.
+    unfold subst_comp_cons in IHE. rewrite IHE; auto. simp subst_eval_context.
+    f_equal. destruct subst_weaken_mid_aux as [? _]. erewrite <- H with (Γ := [t1]); eauto.
+    Unshelve. all : eauto. f_equal. unfold weaken_r_comp, weaken_mid_comp.
+    eapply comp_map_dep_f_equal; eauto. red. intros.
+    cbn in b. dependent destruction b.
+    2 : inversion b1. unfold weaken_var_r. simp append_var. simp weaken_var_mid. auto.
+Qed.
+
+
+Lemma approx_comp_log_rel_bodies_step:
+  forall (R1 R2 : call_frame) (MR : mfix_ctx) (sbodies : mfix_bodies [] MR R1 R2)
+    (dbodies : forall arg : denote_call_frame R2, mtree (denote_mfix_ctx (R1 :: MR)) (encodes arg)) (tin tout : vtype)
+    (x : var (tin, tout) R2) (vvin : denote_type tin) (n : nat) (vcall : closed_value tin),
+    log_rel_bodies_step n dbodies sbodies ->
+    approx_val n tin vvin vcall ->
+    approx_comp (n - 1) approx_val (apply_bodies dbodies x vvin) (subst_comp_cons (nth_body sbodies x) vcall).
+Proof.
+  intros R1 R2 MR sbodies dbodies tin tout x vvin n vcall.
+  intros Hbodies Hin. destruct n. constructor. intros. lia.
+  dependent induction x.
+  - dependent destruction sbodies. simp nth_body. unfold apply_bodies.
+    simp call_mrec_call_frame. setoid_rewrite bind_ret_r.
+    simp log_rel_bodies_step in Hbodies. destruct Hbodies as [Hbody _].
+    simp approx_val in Hbody.
+    specialize (Hbody vvin vcall (S n - 1)).
+    assert (Hn1 : S n - 1 < S n). lia.
+    assert (Hn2 : approx_val (S n - 1) tin vvin vcall). eapply lower_approx_val; try apply Hin. lia.
+    specialize (Hbody Hn1 Hn2). clear - Hbody. revert Hbody.  
+    eapply lower_approx_comp_aux1 with (P := fun n0 => n0 < S n). lia.
+    intros. lia. intros. split; auto.
+  - dependent destruction sbodies. 
+    simp nth_body. simp log_rel_bodies_step in Hbodies.
+    destruct Hbodies as [_ Hbodies].
+    assert (apply_bodies dbodies (VarS x) vvin ≅ apply_bodies (fun x : denote_call_frame l => dbodies (inr x)) x vvin).
+    unfold apply_bodies. simp call_mrec_call_frame. destruct (call_mrec_call_frame x vvin). reflexivity.
+    rewrite H. eapply IHx; eauto.
+Qed.
+
+Lemma call_term_bind_inv_aux1  : 
+ forall (MR : mfix_ctx)
+    (R0 : call_frame) (tin0 tout0 : vtype) (x0 : var (tin0, tout0) R0) (xR0 : var R0 MR)
+    (vvin : denote_type tin0)
+    (tin tout : vtype) (Rcall : call_frame)
+    (xR : var Rcall MR) (x : var (tin, tout) Rcall) (vvcall : denote_type tin),
+   projT1 (call_mrec x xR vvcall) = projT1 (call_mrec x0 xR0 vvin) ->
+   var_eq xR xR0.
+Proof.
+  intros. generalize dependent xR0.
+  dependent induction xR.
+  - simp call_mrec. intros.
+    dependent destruction xR0. constructor. simp call_mrec in H.
+    destruct (call_mrec_call_frame x vvcall). destruct (call_mrec x0 xR0 vvin).
+    discriminate.
+  - intros. dependent destruction xR0.
+    + simp call_mrec in H. destruct (call_mrec x xR vvcall). 
+      destruct (call_mrec_call_frame x0 vvin). discriminate.
+    + constructor. eapply IHxR with (x := x) (vvcall := vvcall).
+      simp call_mrec in H.
+      destruct (call_mrec x xR vvcall). destruct (call_mrec x0 xR0 vvin).
+      injection H. intros. subst. auto.
+Qed.
+
+Lemma call_term_bind_inv_aux2 : 
+ forall (MR : mfix_ctx)
+    
+    (tin tout : vtype) (Rcall : call_frame)
+    (tin0 tout0 : vtype) (x0 : var (tin0, tout0) Rcall)
+    (xR : var Rcall MR) (x : var (tin, tout) Rcall) (vvcall : denote_type tin) 
+    (vvin : denote_type tin0),
+   projT1 (call_mrec x xR vvcall) = projT1 (call_mrec x0 xR vvin) ->
+   (var_eq x x0 * (vvin ~= vvcall))%type.
+Proof.
+  intros. generalize dependent x0. generalize dependent x.
+  dependent induction xR.
+  - intros. simp call_mrec in H.
+    assert (projT1 (call_mrec_call_frame x vvcall) = projT1 (call_mrec_call_frame x0 vvin)).
+    destruct (call_mrec_call_frame x vvcall). destruct (call_mrec_call_frame x0 vvin).
+    injection H. intros. auto. clear H.
+    generalize dependent x0. dependent induction x.
+    + simp call_mrec_call_frame. intros.
+      dependent destruction x0. simp call_mrec_call_frame in H0. injection H0.
+      intros. subst. split; constructor. exfalso.
+      simp call_mrec_call_frame in H0. destruct (call_mrec_call_frame x0 vvin).
+      discriminate.
+    + intros.
+      dependent destruction x0.
+      * simp call_mrec_call_frame in H0. destruct (call_mrec_call_frame x vvcall).
+        discriminate.
+      * destruct b. simp call_mrec_call_frame in H0.
+        enough (var_eq x x0 * (vvin ~= vvcall)). destruct X. split; auto.
+        constructor. auto.
+        eapply IHx; eauto. 
+        destruct (call_mrec_call_frame x vvcall).
+        destruct (call_mrec_call_frame x0 vvin). injection H0. auto.
+  - intros. eapply IHxR. simp call_mrec in H.
+    destruct (call_mrec x xR vvcall).
+    destruct (call_mrec x0 xR vvin). injection H. intros. subst.
+    auto.
+Qed.
+
+
+Lemma call_term_bind_inv1:
+  forall (t : vtype) (MR : mfix_ctx)
+    (R0 : call_frame) (tin0 tout0 : vtype) (x0 : var (tin0, tout0) R0) (xR0 : var R0 MR)
+    (vvin : denote_type tin0)
+    (k1 : denote_type tout0 -> mtree (denote_mfix_ctx (MR)) (denote_type t)) 
+    (tin tout : vtype) (Rcall : call_frame)
+    (xR : var Rcall MR) (x : var (tin, tout) Rcall) (vvcall : denote_type tin)
+    (k' : denote_type tout -> mtree (denote_mfix_ctx (MR)) (denote_type t)) b1 b2,
+    eqit eq b1 b2 (vv <- call_term x xR vvcall;; (k' vv)) (vv <- call_term x0 xR0 vvin;; (k1 vv)) ->
+    tin = tin0 /\ tout = tout0 /\ x ~= x0 /\ xR ~= xR0 /\ Rcall = R0 /\ vvcall ~= vvin.
+Proof.
+  intros t MR R0 tin0 tout0 x0 xR0 vvin k1 tin tout Rcall xR x vvcall k'.
+  unfold call_term. destruct (call_mrec x xR vvcall) eqn : Heq1.
+  destruct (call_mrec x0 xR0 vvin) eqn : Heq2. setoid_rewrite bind_trigger.
+  setoid_rewrite bind_vis. 
+  intros. assert (x1 = x2). pinversion H. auto. subst.
+  specialize (eqit_Vis_inv _ _ _ _ _ _ H) as H'. setoid_rewrite bind_ret_l in H'.
+  clear H H'. 
+  assert (var_eq xR xR0).
+  { eapply call_term_bind_inv_aux1. rewrite Heq1, Heq2. auto. }
+  apply var_eq_surj in X as ?. subst. apply var_eq_eq in X. subst.
+  assert ((var_eq x x0 * (vvin ~= vvcall))%type).
+  eapply call_term_bind_inv_aux2. rewrite Heq1, Heq2. auto.
+  destruct X as [Heq HJMeq]. apply var_eq_surj in Heq as ?. injection X.
+  intros. subst. rewrite HJMeq. apply var_eq_eq in Heq.  subst.
+  repeat split; auto.
+Qed.
+
+Lemma call_term_bind_inv_JMeq_aux :
+forall (t : vtype) (MR : mfix_ctx) A B
+  (k1 k2 : B -> mtree (denote_mfix_ctx MR) (denote_type t))
+  (d : A -> B)
+  (x0 : B) b1 b2 ,
+  (forall x , eqit eq b1 b2 (k1 (d x)) (k2 (d x))) ->
+  d ~= @id B -> A = B -> eqit eq b1 b2 (k1 x0)  (k2 x0).
+Proof.
+  intros. subst. rewrite H0 in H. unfold id in *. auto.
+Qed.
+
+Lemma call_term_bind_inv2:
+  forall (t : vtype) (MR : mfix_ctx)
+    (tin tout : vtype) (Rcall : call_frame)
+    (xR : var Rcall MR) (x : var (tin, tout) Rcall) (vvcall : denote_type tin)
+    (k1 k2 : denote_type tout -> mtree (denote_mfix_ctx MR) (denote_type t)) b1 b2,
+    eqit eq b1 b2 (vv <- call_term x xR vvcall;; (k1 vv))  (vv <- call_term x xR vvcall;; (k2 vv)) ->
+    forall x, eqit eq b1 b2 (k1 x) (k2 x).
+Proof.
+  unfold call_term. intros. destruct (call_mrec x xR vvcall) eqn : Heq1.
+  setoid_rewrite bind_trigger in H. setoid_rewrite bind_vis in H.
+   specialize (call_mrec_encodes _ _ _ _ x xR vvcall) as Henc.
+  specialize (call_mrec_cont _ _ _ _ x xR vvcall) as Hcont.
+  rewrite Heq1 in Hcont. cbn in Hcont. rewrite Heq1 in Henc. cbn in Henc.
+  assert (forall x, eqit eq b1 b2 (k1 (d x)) (k2 (d x))). intros. eapply eqit_Vis_inv in H.
+  setoid_rewrite bind_ret_l in H. eauto. eapply call_term_bind_inv_JMeq_aux; eauto.
+Qed.
+ 
+(*
+Lemma mfix_compat t Γ R MR dbodies sbodies m (c : comp t Γ (R :: MR)):
+  bodies_rel dbodies sbodies ->
+  comp_rel m c ->
+  comp_rel (interp_mrec_bodies dbodies m) (comp_mfix _ sbodies c).
+
+*)
+
+(* use the trick from bind_compat to get a useful inductive hypothesis *)
+Lemma mfix_compat_aux n : forall t Γ R MR dbodies sbodies m (c : comp t Γ (R :: MR)),
+  bounded_bodies_rel n dbodies sbodies ->
+  bounded_comp_rel n m c ->
+  bounded_comp_rel n (interp_mrec_bodies dbodies m) (comp_mfix _ sbodies c).
+Proof.
+  induction n as [n00 IHn] using (well_founded_induction lt_wf).
+  intros t Γ R MR dbodies sbodies m c Hbodies Hmc n hyps ρ Hnn Hhρ. 
+  constructor. intros. split.
+  - intros vv Hvv. apply recursion_trace_den_ret in Hvv as Hvv'.
+    destruct Hvv' as [l Hrec].
+    red in Hmc.
+    specialize (Hmc n hyps ρ Hnn Hhρ).
+    (**)
+    unfold interp_mrec_bodies in Hvv. rewrite close_comp_mfix. red in Hbodies.
+    specialize (Hbodies n hyps ρ Hnn Hhρ).
+    remember (close_comp Γ ρ c) as c'. remember (close_bodies Γ ρ sbodies) as sbodies'.
+    remember (dbodies hyps) as dbodies'. remember (m hyps) as m'.
+    clear Heqsbodies' Heqdbodies' Heqc' Heqm'. clear m sbodies c dbodies.
+    clear Hvv Hhρ ρ hyps Γ. revert Hmc. generalize dependent c'.
+    remember (ret vv) as x. revert Heqx. generalize dependent n. induction Hrec; intros.
+    (* now I am back to feeling confident this is the correct relation,
+       but I suspect I am not at the exact correct generality 
+     *)
+    + subst. apply eqit_Ret_inv in H. subst.
+      rewrite H0 in Hmc. inversion Hmc. subst.
+      assert (H00 : 0 < n0). lia.
+      specialize (H _ H00). destruct H as [Hret _].
+      assert (multi_step (E := denote_mrec_ctx (denote_mfix_ctx (R :: MR))) 0 (ret r) (ret r)).
+      constructor. reflexivity. specialize (Hret _ H).
+      destruct Hret as [v [Hv1 Hv2]].
+      exists v. split.
+      * apply eval_rel_stuck_mfix_ret; auto.
+      * eapply lower_approx_val'; try apply Hv2. lia.
+    + exfalso. subst. clear - H. unfold call_term in H.
+      destruct (call_mrec x xR vvin). setoid_rewrite bind_trigger in H.
+      setoid_rewrite bind_vis in H. pinversion H.
+    + subst. rewrite H in Hmc. specialize (IHHrec (n0 - 1)). 
+      assert (Hbodiesn0 : log_rel_bodies_step (n0 - 1) dbodies' sbodies').
+      eapply lower_log_rel_bodies_step; try apply Hbodies. lia.
+      assert (Hn0 : n < n0 - 1). lia.
+      assert (Hn00 : n0 - 1 <= n00). lia.
+      specialize (IHHrec Hbodiesn0 Hn00 Hn0 eq_refl).
+      inversion Hmc. subst. assert (H00 : 0 < n0). lia.
+      specialize (H1 0 H00). destruct H1 as [_ Hstuck].
+      assert (H2 : multi_step 0 (vv <- call_term x VarZ vvin;; k1 vv) (vv <- call_term x VarZ vvin;; k1 vv)).
+      constructor. reflexivity. specialize (Hstuck _ _ _ _ _ _ _ H2).
+      destruct Hstuck as [vcall [E [c'' [HE1 [HE2 [HE3 HE4 ]]]]]].
+      set (subst_eval_context E (subst_comp_cons (nth_body sbodies' x) vcall)) as c'''.
+      specialize (IHHrec c''').
+      assert (approx_comp (n0 - 1) approx_val (x <- apply_bodies dbodies' x vvin;; k1 x) c''').
+      {
+        unfold c'''.
+        eapply approx_comp_eval_context; eauto.
+        - eapply  approx_comp_log_rel_bodies_step; eauto.
+          eapply lower_approx_val'; try apply HE1. lia.
+        - intros. apply HE4; auto. lia.
+      }
+      specialize (IHHrec H1). destruct IHHrec as [v [Hv1 Hv2]].
+      exists v. split.
+      * eapply eval_rel_stuck_mfix_stuck_call_VarZ; eauto. 
+      * eapply lower_approx_val'; try apply Hv2. lia.
+    + intros. subst. specialize (IHHrec (n0 - n)).
+      assert (Hmn0 : m < n0 - n). lia.
+      assert (Hbodiesn0 : log_rel_bodies_step (n0 - n) dbodies' sbodies').
+      eapply lower_log_rel_bodies_step'; try apply Hbodies. lia.
+      assert (Hnn0 : n0 - n <= n00). lia.
+      specialize (IHHrec Hbodiesn0 Hnn0 Hmn0 eq_refl). specialize (IHHrec c').
+      match type of IHHrec with | ?P1 -> ?P2 => enough P1 end.
+      specialize (IHHrec H1). destruct IHHrec as [v [Hv1 Hv2]].
+      eexists. split; eauto. eapply lower_approx_val'; try apply Hv2.
+      lia. eapply approx_comp_multi_step_minus; eauto. lia.
+  - intros ? ? ? ? ? ? ? Hstep. unfold interp_mrec_bodies in *.
+    setoid_rewrite close_comp_mfix. 
+    eapply multi_step_interp_mrec_den_vis_inv in Hstep as Hk'.
+    destruct Hk' as [k' Hk']. setoid_rewrite Hk' in Hstep.
+    setoid_rewrite Hk'. clear Hk' k. red in Hmc.
+    specialize (Hmc n hyps ρ Hnn Hhρ).
+    specialize (Hbodies n _ _ Hnn Hhρ).
+    remember (close_comp Γ ρ c) as c'. remember (close_bodies Γ ρ sbodies) as sbodies'.
+    remember (dbodies hyps) as dbodies'. remember (m hyps) as m'.
+    eapply recursion_trace_den_vis in Hstep. destruct Hstep as [l Hrec].
+    clear Heqsbodies' Heqdbodies' Heqc' Heqm'. clear m sbodies c dbodies.
+    clear Hhρ ρ hyps Γ.  generalize dependent c'. generalize dependent n.
+    dependent induction Hrec; intros.
+    + clear - H. exfalso. unfold call_term in H.
+      destruct (call_mrec x xR vvcall). setoid_rewrite bind_trigger in H.
+      setoid_rewrite bind_vis in H. pinversion H.
+    + intros. setoid_rewrite H0 in Hmc. 
+      eapply call_term_bind_inv1 in H as H1'. destruct H1' as [? [? [? [? [? ?]]]]]. 
+      subst. subst. 
+      assert (forall x, interp_mrec dbodies' (k' x) ≅ interp_mrec dbodies' (k1 x)).
+      eapply call_term_bind_inv2; eauto.
+      inversion Hmc. subst. assert (H00 : 0 < n0). lia.
+      specialize (H3 0 H00). destruct H3 as [_ Hstuck].
+      specialize (Hstuck tin0 tout0 _ (VarS xR0) x0 vvin k1).
+      assert (multi_step 0 (vv <- call_term x0 (VarS xR0) vvin;; k1 vv)
+             (vv <- call_term x0 (VarS xR0) vvin;; k1 vv)). constructor. reflexivity.
+      specialize (Hstuck H3).
+      destruct Hstuck as [vcall [E [c'' [HE1 [HE2 [HE3 HE4]]]]]].
+      specialize stuck_call_push_eval_context_mfix. intros HE'. 
+      specialize (HE' _ _ _ _ sbodies' _ _ _ _ _ E).
+      destruct HE' as [E' [HE'1 HE'2]].
+      (* need more properties of E' *)
+      exists vcall. 
+      exists E'.
+      exists (push_eval_context _ E (comp_mfix_map sbodies') (comp_call xR0 x0 vcall)).
+      split; [ | split; [ | split]].
+      * eapply lower_approx_val'; try apply HE1. lia.
+      * eapply eval_rel_stuck_mfix_stuck_call_neq_VarZ; eauto.
+        eapply eval_rel_stuck_stuck; eauto.
+      * eauto.
+      * intros. setoid_rewrite H2.
+        eapply approx_comp_approx_comp_term; eauto.
+        assert (Hj'' : j'' < n00). lia.
+        specialize (IHn j'' Hj'' t [] R MR (fun _ => dbodies') sbodies'). 
+        specialize (IHn (fun _ => (k1 vvret)) (subst_eval_context E (comp_ret vret))).
+        assert (bounded_bodies_rel j'' (fun _ : denote_ctx [] => dbodies') sbodies').
+        red. intros j [] [] ? ?. simp close_bodies. 
+        eapply lower_log_rel_bodies_step'; try apply Hbodies. lia.
+        specialize (IHn H6).
+        match type of IHn with | ?P1 -> ?P2 => assert P1 end.
+        red. intros j [] [] ? ?. simp close_comp.
+        eapply lower_approx_comp'; try apply HE4; eauto. 
+        intros.
+        eapply lower_approx_val; eauto. lia.
+        specialize (IHn H7). red in IHn. 
+        specialize (IHn j'' tt tt (le_n _) (closing_subst_approx_nil _)).
+        simp close_comp in IHn.
+    + subst. rewrite H in Hmc. 
+      specialize (IHHrec IHn). specialize (IHHrec _ _ _ xR x vvcall k').
+      assert (H00 : vv <- call_term x xR vvcall;; interp_mrec dbodies' (k' vv) =
+           vv <- call_term x xR vvcall;; interp_mrec dbodies' (k' vv)).
+      reflexivity.
+      specialize (IHHrec H00). 
+      inversion Hmc. subst. specialize (H1 0). 
+      clear H00. assert (H00 : 0 < n0). lia.
+      specialize (H1 H00). destruct H1 as [_ Hstuck].
+      assert (Hstep0 : multi_step 0 (vv <- call_term x0 VarZ vvin;; k1 vv) 
+                                  (vv <- call_term x0 VarZ vvin;; k1 vv)).
+      constructor. reflexivity.
+      apply Hstuck in Hstep0. clear Hstuck.
+      destruct Hstep0 as [vcall [E [c'' [HE1 [HE2 [HE3 HE4]]]]]].
+      set (subst_eval_context E (subst_comp_cons (nth_body sbodies' x0) vcall)) as c'''.
+      assert (Hbodiesn0 : log_rel_bodies_step (n0 - 1) dbodies' sbodies').
+      eapply lower_log_rel_bodies_step; try apply Hbodies. lia.
+      assert (Hn0 : n < n0 - 1). lia.
+      assert (Hnn0 : n0 - 1 <= n00). lia.
+      specialize (IHHrec _ Hbodiesn0 Hnn0 Hn0 c''').
+      assert (approx_comp (n0 - 1) approx_val (x <- apply_bodies dbodies' x0 vvin;; k1 x) c''').
+      {
+        unfold c'''. 
+        eapply approx_comp_eval_context; eauto.
+        - eapply approx_comp_log_rel_bodies_step; eauto.
+          eapply lower_approx_val'; try apply HE1. lia.
+        - intros. eapply HE4. lia. auto.
+      }
+      specialize (IHHrec H1).
+      destruct IHHrec as [vcall' [E' [c'''' [HE'1 [HE'2 [HE'3 HE'4]]]]]].
+      unfold c''' in *. exists vcall', E', c''''.
+      split; [ | split; [ | split]].
+      * eapply lower_approx_val'; try apply HE'1. lia.
+      * eapply eval_rel_stuck_mfix_stuck_call_VarZ; eauto.
+      * auto.
+      * intros. eapply HE'4; eauto. lia.
+    + specialize (IHHrec IHn _ _ _ _ _ _ _ eq_refl). 
+      specialize (IHHrec (n0 - n)).
+      assert (Hmn0 : m < n0 - n). lia.
+      assert (Hnn0 : n0 - n <= n00). lia.
+      assert (Hbodiesn0 : log_rel_bodies_step (n0 - n) dbodies' sbodies').
+      eapply lower_log_rel_bodies_step'; try apply Hbodies. lia.
+      specialize (IHHrec Hbodiesn0 Hnn0 Hmn0 c').
+      assert (Happrox : approx_comp (n0 - n) approx_val t2 c').
+      eapply approx_comp_multi_step_minus; eauto. lia.
+      specialize (IHHrec Happrox).
+      destruct IHHrec as [vcall [E [c'' [HE1 [HE2 [HE3 HE4]]]]]].
+      exists vcall, E, c''.
+      split; [ | split; [ | split]]; eauto.
+      * eapply lower_approx_val'; try apply HE1. lia.
+      * intros. eapply HE4; eauto. lia.
+Qed.
+
 Lemma mfix_compat t Γ R MR dbodies sbodies m (c : comp t Γ (R :: MR)):
   bodies_rel dbodies sbodies ->
   comp_rel m c ->
   comp_rel (interp_mrec_bodies dbodies m) (comp_mfix _ sbodies c).
 Proof.
-  intros Hbodies Hmc n hyps ρ Hhρ.
-  constructor. intros. split.
-  - intros vv Hvv. apply recursion_trace_ret in Hvv as Hvv'.
-    destruct Hvv' as [l Hrec].
-    specialize (Hmc n _ _ Hhρ).
-    (**)
-    unfold interp_mrec_bodies in Hvv.
-    generalize dependent (m hyps). generalize dependent c.
-    clear m.
-    (*Hhρ is a little problematic, could get rid of it if I can commute close_comp with 
-      comp_mfix *)
-    (* will require a bind lemma *)
-    induction j' as [ j IHj ] using (well_founded_induction lt_wf).
-    intros c m Happrox Hstep Hrec. dependent destruction Hrec.
-    + admit.
-    + admit.
-    +
-    
-    revert Happrox Hstep.
-    dependent induction Hrec.
-    + intros. setoid_rewrite H2 in Hstep. 
-      inversion Happrox. subst. assert (0 < n). lia. specialize (H0 0 H1).
-      destruct H0 as [Hret _].
-      setoid_rewrite H2 in Hret. assert (r = vv). apply eqit_Ret_inv in H3. subst. auto.
-      subst. specialize (Hret vv). 
-      assert (multi_step (E := denote_mrec_ctx (denote_mfix_ctx (R :: MR))) 0 (ret vv) (ret vv)).
-      constructor. reflexivity. specialize (Hret H0).
-      destruct Hret as [v [Hv1 Hv2]]. exists v.
-      split.
-      * (*step metatheory*) admit.
-      * destruct n0; auto. eapply lower_approx_val; try apply Hv2. lia.
-    + exfalso. (* ret ≅ vis*) admit.
-    +
+  intros. red. intros. eapply mfix_compat_aux; eauto.
+  all : red; intros; eauto.
+Qed.
 
+Lemma call_compat tin tout Γ R MR m (vin : value tin Γ) 
+      (xR : var R MR) (x : var (tin, tout) R) :
+  val_rel m vin ->
+  comp_rel (fun hyps => vvin <- m hyps;; call_term x xR vvin) (comp_call xR x vin).
+Proof.
+  intros Hval. red. intros.
+  apply Hval in H as Hval'. destruct Hval' as [vvin [Hvvin1 Hvvin2]].
+  setoid_rewrite Hvvin1. setoid_rewrite bind_ret_l.
+  constructor. intros.
+  split.
+  - intros. exfalso. apply multi_step_eutt in H1. unfold call_term in H1.
+    destruct (call_mrec x xR vvin). setoid_rewrite bind_vis in H1. pinversion H1.
+  - intros. apply multi_step_eutt in H1 as H1'.
+    setoid_rewrite <- bind_ret_r with (s := call_term x xR vvin) in H1'.
+    apply call_term_bind_inv1 in H1' as H2. decompose record H2. subst. subst. clear H2.
+    clear H1'. dependent destruction H1.
+    2 : { dependent destruction H3. unfold call_term in H2. 
+          destruct (call_mrec x0 xR0 vvcall). setoid_rewrite bind_vis in H2.
+          pinversion H2. inversion CHECK. }
+    setoid_rewrite <- bind_ret_r with (s := call_term x0 xR0 vvcall) in H1 at 1.
+    assert (forall x, k x ≅ ret x). intros. symmetry. eapply call_term_bind_inv2;  eauto.
+    setoid_rewrite H2. exists (close_value Γ ρ vin), ev_hole, (comp_call xR0 x0 (close_value Γ ρ vin)).
+    split; [ | split; [ | split]].
+    + eapply lower_approx_val'; try apply Hvvin2. lia.
+    + rewrite close_comp_call.
+      eapply eval_rel_stuck_stuck. constructor.
+    + constructor.
+    + intros. simp subst_eval_context. constructor.
+      intros. split.
+      * intros. apply multi_step_eutt in H6.
+        apply eqit_Ret_inv in H6. subst. exists vret.
+        split. apply eval_rel_stuck_val. unfold step. simp observe. auto.
+        eapply lower_approx_val'; try apply H4. lia.
+      * intros. exfalso. clear - H6. apply multi_step_eutt in H6.
+        unfold call_term in H6. destruct (call_mrec x xR vvcall0).
+        setoid_rewrite bind_trigger in H6. setoid_rewrite bind_vis in H6.
+        pinversion H6.
+Qed.
 
-    destruct Hvv as [l Hrec]. 
-    assert (approx_comp (n + length l) approx_val (m hyps) (close_comp Γ ρ c)).
-    apply Hmc. 
+(* note that you added this tau during the application, will need to be added to the
+   denotation *)
+Lemma app_compat t1 t2 Γ MR mf marg (vf : value (Arrow t1 MR t2) Γ)
+      (varg : value t1 Γ) : 
+  val_rel mf vf ->
+  val_rel marg varg ->
+  comp_rel (fun hyps => vvf <- mf hyps;; vvarg <- marg hyps;; Tau (vvf vvarg)) 
+           (comp_app vf varg).
+Proof.
+  intros Hf Harg. intros n hyps ρ Hhρ.
+  specialize (Hf n _ _ Hhρ). specialize (Harg n _ _ Hhρ).
+  destruct Hf as [vvf [Hvvf1 Hvvf2]].
+  destruct Harg as [vvarg [Hvvarg1 Hvvarg2]].
+  rewrite Hvvf1. setoid_rewrite bind_ret_l.
+  rewrite Hvvarg1. setoid_rewrite bind_ret_l.
+  destruct n. constructor. intros. lia.
+  rewrite close_comp_comp_app.
+  remember (close_value Γ ρ vf) as vf'. clear Heqvf' vf.
+  remember (close_value Γ ρ varg) as varg'. clear Heqvarg' varg.
+  dependent destruction vf'; try inversion x.
+  simp approx_val in Hvvf2.
+  eapply approx_comp_multi_step_1. econstructor.
+  constructor. reflexivity. constructor. reflexivity.
+  eapply approx_comp_approx_comp_term; try apply approx_comp_term_comp_call.
+  eapply lower_approx_comp_aux1 with (P := fun m' => m' < S n); try eapply Hvvf2; try lia.
+  2 : eapply lower_approx_val; try apply Hvvarg2; try lia.
+  intros. split; auto.
+Qed.
 
-    (* this is a major problem in order to use Hmc at n + len lI need to know the contexts approx 
-                 each other at n + len l but I only know that for n
-                 maybe this is the wrong level of abstraction, could I prove some core part of this lemma 
-                 on closed terms and then use that to generalize?
-     *)
-    (* needs to be rutt, do that today?
-    eapply recursion_trace_den_ret in Hvv.
-    *)
+Lemma abs_compat t1 t2 MR MR' Γ m (cbody : comp t2 (t1 :: Γ) MR) :
+  comp_rel m cbody ->
+  val_rel (MR := MR') (fun hyps => ret (fun x => m (x, hyps))) (val_abs cbody).
+Proof.
+  intros. econstructor. split. reflexivity.
+  rewrite close_value_abs. destruct n; simp approx_val; auto.
+  intros. specialize (H m' (vv,hyps) (v,ρ)). 
+  assert (Hhρ' : closing_subst_approx m' (t1 :: Γ) (vv, hyps) (v, ρ)).
+  constructor. auto. eapply lower_closing_subst_approx; eauto.
+  specialize (H Hhρ'). rewrite <- close_comp_open.
+  eapply lower_approx_comp_aux1 with (P := fun m' => m' < S n); try lia; eauto.
+  split; intros; auto.
+Qed.
 
+Lemma const_compat MR Γ (n : nat) :
+  val_rel (MR := MR) (fun hyps : denote_ctx Γ => ret n) (val_const n).
+Proof.
+  econstructor. split. reflexivity. rewrite close_value_const. 
+  destruct n0; simp approx_val; auto.
+Qed.
 
-
-(*
-IH : forall m l vv, recursion_trace_den m l (ret vv) ->
-     forall c, m <=(n + len l) c ->
-       exists v, mfix bodies c ->* v /\ vv <=n v
-
-
-   Base case : 
-     m ≈ ret vv
-     which means (ret vv) <=(n + len l) c so
-     c ->* v where vv <=(n + len) v going the rest of the way is trivial assuming lemmas that should hold
-
-
-   Inductive case :
-    H1:m1 ≈ (vv <- call_term vvin;; k1 vv)
-    H2:recursion_trace (vv <- (apply_bodies x vvin);; k1 vv ) l m3
-    H3: m1 <=(n + len l + 1) c
-
-    using H1 and H3 can learn that c ->* E[ca] where vvin <=(n + len l + 1) ca
-
-
-    enough to show exists v, mfix bodies E[ca] ->* v /\ vv <=n v
-
-    which I can prove using IH and a proof that vv <- (apply_bodies x vvin);; k1 vv <=(n + len l) E[ca]
-
-    Intuitively this should be true and derivable from H1, H3 and the fact that c ->* E[ca]
-    is this the equivalent of the lemma nick suggested? I feel like it might be look into this carefully
-
-
-    two parts 
-    1 : m <=n c and c ->* E[ca] then m <=n E[ca] ( probably wrong generality)
-    2 : call_term vvin;; k <=n E[ca] ->
-
-                  forall j, bodies vvin <=j c -> 
-                         bodies vvin;; k <=(n - 1) let x = c1 in E[x]  (or is it at n + 1? that is strictly stronger)
-                         ??? probably bugs in this statement maybe it is backwards, but I think the idea that removing a call lowers a step index seems sound
-                         also might rely on bodies approximating a syntax at all levels
-
-
-*)
+Lemma var_compat MR Γ t (x : var t Γ) :
+  val_rel (MR := MR) (fun hyps : denote_ctx Γ => ret (index_ctx x hyps)) (val_var x).
+Proof.
+  red. intros. eexists. split. reflexivity.
+  generalize dependent Γ. intros Γ x. dependent induction x.
+  - intros [vv hyps] [v ρ] H. dependent destruction H. simp index_ctx. simp close_value.
+    unfold subst_value_cons. simp subst_comp. simp subst_var.
+    assert (close_value l ρ (weaken_r_value l v) = v).
+    { (* this contains a few things that could be lifted out as lemmas *)
+      generalize dependent l. clear H. intros Γ. revert v.
+      induction Γ.
+      - intros. simp close_value. unfold weaken_r_value. rewrite val_map_id; auto.
+        intros. inversion x.
+      - intros v [vv' hyps] [v' ρ] H. dependent destruction H.
+        eapply IHΓ with (v := v)in H0. simp close_value.
+        generalize dependent ρ. induction Γ.
+        + intros []. simp close_value. intros. unfold subst_value_cons. 
+          rewrite subst_value_weaken_r. auto.
+        + intros [v'' ρ] H'. simp close_value in H'.
+          simp close_value. rewrite <- H' at 2. f_equal.
+          f_equal.
+          destruct subst_weaken_mid_aux as [_ [Hmid _]].
+          erewrite <- Hmid with (v1' := weaken_r_value (a1 :: Γ) v) (t2 := a0) (v2 := (weaken_r_value (a1 :: Γ) v')); eauto.
+          unfold subst_value_cons. f_equal. unfold weaken_r_value, weaken_mid_value.
+          rewrite val_map_fusion. eapply val_map_dep_f_equal; auto.
+          red. intros. inversion b.
+    }
+    rewrite H1. auto.
+  - intros [vv hyps] [v ρ] H. dependent destruction H. simp index_ctx. simp close_value.
+    unfold subst_value_cons. simp subst_comp. simp subst_var. apply IHx in H0.
+    destruct l. inversion x.
+    simp subst_var.
+Qed.
