theories/AlmostStlc/SmallStepSeqFacts.v
@@ -2,10 +2,16 @@ Require Export TypedVar.
 Require Export SyntaxSeq.
 Require Export SmallStepSeq.
 Require Export SemanticsFactsSeq.
+Require Export SemanticsFactsSeq2.
+Require Export ClosingSubst.
 Import List.ListNotations.
 Open Scope list_scope.
 From Equations Require Import Equations Signature.
 Require Import Coq.Program.Equality.
+Require Import Lia.
+
+
+
 
 Lemma step_ret t MR (v : closed_value t) :
   step (MR := MR) (comp_ret v) = inr v.
@@ -14,7 +20,7 @@ Proof.
 Qed.
 
 
-Lemma step_let t1 t2 MR (c1 c1' : comp t1 [] MR) (c2 : comp t2 [t1] MR) :
+Lemma step_let1 t1 t2 MR (c1 c1' : comp t1 [] MR) (c2 : comp t2 [t1] MR) :
   step_rel c1 c1' ->
   step_rel (comp_let c1 c2) (comp_let c1' c2).
 Proof.
@@ -28,52 +34,422 @@ Proof.
   - simp step_eval_context. cbn. injection H. intros. rewrite H0. auto.
 Qed.
 
-(* probably the most complicated one
-   covered_in SemanticsFactsSeq.v might be a useful abstraction
-   keep an eye out for counter example,
-   maybe it evaluates in a different order than you are thinking
-   figure out what the boolean in step_eval_context is
 
-   still pretty confident it should be true, but should also consider
-   what related property might be true
-*)
-Locate step_eval_context.
+Lemma step_let2 t1 t2 MR (c1 : comp t1 [] MR) (c2 : comp t2 [t1] MR) (v1 : closed_value t1) :
+  step c1 = (inr v1) -> step_rel (comp_let c1 c2) (subst_comp_cons c2 v1).
+Proof.
+  intros. econstructor. unfold step. simp observe. unfold step in H.
+  destruct (SmallStepSeq.observe c1); try destruct b;
+    try discriminate. cbn. simp step_eval_context. f_equal. simpl Monad.ret.
+  simp step_bredex. simp subst_eval_context. injection H. intros. subst. auto.
+Qed.
+
+Equations num_lets {t Γ MR} (c : comp t Γ MR) : nat :=
+  num_lets (comp_ret v) := 0;
+  num_lets (comp_let c1 c2) := 1 + num_lets c1 + num_lets c2;
+  num_lets (comp_match_nat vn c1 c2) := num_lets c1 + num_lets c2;
+  num_lets (comp_succ vn) := 0;
+  num_lets (comp_match_list vl c1 c2) := num_lets c1 + num_lets c2;
+  num_lets (comp_split vp cs) := num_lets cs;
+  num_lets (comp_app vf varg) := 0;
+  num_lets (comp_call _ _ _) := 0;
+  num_lets (comp_mfix R bodies c) := num_lets c;
+  num_lets (comp_lift c) := num_lets c;
+  num_lets (comp_perm _ c) := num_lets c.
+
+Transparent num_lets.
+
+Lemma num_lets_subst_comp MR t1 Γ1 t2 Γ2 (c : comp t1 (Γ1 ++ [t2] ++ Γ2) MR)
+      (v : value t2 Γ2) :
+  num_lets c = num_lets (subst_comp c v).
+Proof.
+  dependent induction c; simp subst_comp; simp num_lets; auto.
+  - erewrite IHc1 with (v := v); eauto. f_equal.
+    eapply IHc2 with (Γ1 := t1 :: Γ1); auto.
+  - erewrite IHc1 with (v := v); eauto. f_equal.
+    eapply IHc2 with (Γ1 := Nat :: Γ1); auto.
+  - erewrite IHc1 with (v := v); eauto. f_equal.
+    eapply IHc2 with (Γ1 := _ :: _ :: Γ1); auto.
+  - eapply IHc with (Γ1 := _ :: _ :: Γ1); auto.
+Qed.
+
+(* remaining cases should be similarly easy *)
+
+Lemma step_let3 t1 t2 MR (c1 c1' : comp t1 [] MR) (c2 : comp t2 [t1] MR) :
+  step_rel (comp_let c1 c2) (comp_let c1' c2) ->
+  step_rel c1 c1'.
+Proof.
+  intros. dependent destruction H. constructor. unfold step. unfold step in H.
+  simp observe in H. destruct (SmallStepSeq.observe c1) eqn : Heqx; try destruct b;
+    try discriminate.
+  - destruct r; simp step_eval_context in H.
+    + cbn in H. simp step_eval_context. cbn. simp subst_eval_context in H.
+      injection H. intros. inj_existT. rewrite H0. auto.
+    + cbn in H. destruct (step_eval_context b (inr c) E).
+      injection H. intros. inj_existT. subst. auto.
+      discriminate.
+  - rename c into v.
+    cbn in H. simp step_eval_context in H. cbn in H. simp subst_eval_context in H.
+    simp step_bredex in H. injection H. intros. exfalso.
+    assert (num_lets (subst_comp_cons c2 v) = num_lets (comp_let c1' c2)).
+    rewrite H0. auto. simp num_lets in H1. 
+    unfold subst_comp_cons in H1. 
+    rewrite <- num_lets_subst_comp with (Γ1 := []) (t2 := t1) (Γ2 := []) in H1.
+    clear - H1. assert (1 + num_lets c1' + num_lets c2 > num_lets c2). lia.
+    rewrite H1 in H at 2. lia.
+Qed.
+
+Lemma step_let4 t1 t2 MR (c1 : comp t1 [] MR) (c2 : comp t2 [t1] MR) c3 :
+  step_rel (comp_let c1 c2) c3 ->
+  (exists v, c1 = comp_ret v /\ c3 = subst_comp_cons c2 v) \/ (exists c1', c3 = comp_let c1' c2).
+Proof.
+  intros H. dependent destruction H. unfold step in H.
+  simp observe in H. destruct (SmallStepSeq.observe c1) eqn : Heqx; try destruct b.
+  - destruct r; simp step_eval_context in H. cbn in H. injection H. intros. subst.
+    simp subst_eval_context. right. eexists. eauto.
+    cbn in H. injection H. intros. destruct (step_eval_context b (inr c) E).
+    injection H0. intros. subst. right. eexists. eauto.
+    discriminate.
+  - left. dependent destruction c1; simp observe in Heqx; try discriminate.
+    + injection Heqx. intros. subst. cbn in H. simp step_eval_context in H. 
+      cbn in H. simp subst_eval_context in H. simp step_bredex in H.
+      injection H. intros. subst. eexists. split; eauto.
+    + destruct (SmallStepSeq.observe c1_1); try destruct b; discriminate.
+    + dependent destruction vn; try inversion x. simp observe in Heqx.
+      discriminate.
+    + dependent destruction vn; try inversion x. simp observe in Heqx.
+      discriminate.
+    + dependent destruction vf; try inversion x. simp observe in Heqx.
+      discriminate.
+    + destruct (SmallStepSeq.observe c1); try destruct b; discriminate.
+    + destruct (SmallStepSeq.observe c1); try destruct b; discriminate.
+    + destruct (SmallStepSeq.observe c1); try destruct b; discriminate.
+Qed.
+
+Lemma step_let5 t1 t2 MR (c1 : comp t1 [] MR) (c2 : comp t2 [t1] MR) c3 :
+  step_rel (comp_let c1 c2) c3 ->
+  (exists v, c1 = comp_ret v /\ c3 = subst_comp_cons c2 v) \/ (exists c1', c3 = comp_let c1' c2 /\ step_rel c1 c1').
+Proof.
+  intros. eapply step_let4 in H as H'. destruct H'.
+  - left. auto.
+  - right. destruct H0 as [c1' Hc1']. 
+    subst. eexists. split; auto. eapply step_let3; eauto.
+Qed.
+
+
+Lemma eval_rel_stuck_ex_call t MR (c1 c2 : comp t [] MR) :
+  eval_rel_stuck c1 (inr c2) ->
+  exists t' (ca : call_syn t' MR) (E : eval_context t MR (inr ca) true), stuck_call c2 ca E.
+Proof.
+  intros H. dependent induction H; eauto.
+Qed.
+
+Lemma stuck_call_inj t1 t2 t3 MR (c : comp t1 [] MR)
+      (ca1 : call_syn t2 MR) (ca2 : call_syn t3 MR) E1 E2 :
+  stuck_call c ca1 E1 -> stuck_call c ca2 E2 ->
+  t2 = t3 /\ ca1 ~= ca2 /\ E1 ~= E2.
+Proof.
+  intros H. dependent induction H.
+  - intros. dependent destruction H0.
+    eapply IHstuck_call in H0. destruct H0 as [? [? ?]]. subst. auto.
+  - intros. dependent destruction H. auto.
+Qed.
+
+Lemma eval_rel_stuck_inj t MR (c1 c2 c3 : comp t [] MR) :
+  eval_rel_stuck c1 (inr c2) ->
+  eval_rel_stuck c1 (inr c3) ->
+  c2 = c3.
+Proof.
+  intro H. generalize dependent c3.
+  dependent induction H.
+  - intros. dependent destruction H1.
+    + dependent destruction H. dependent destruction H1.
+      rewrite H in H1. injection H1. intros. subst. eapply IHeval_rel_stuck in H2; eauto.
+    + apply stuck_call_stuck' in H1. dependent destruction H.
+      rewrite H in H1. discriminate.
+  - intros. dependent destruction H0.
+    + apply stuck_call_stuck' in H. dependent destruction H0.
+      rewrite H in H0. discriminate.
+    + auto.
+Qed.
+
+
+Lemma eval_rel_stuck_let1 t1 t2 MR (c1 : comp t1 [] MR) (c2 : comp t2 [t1] MR)
+      (v1 : closed_value t1) (r : closed_value t2 + comp t2 [] MR) : 
+  eval_rel_stuck c1 (inl v1) -> eval_rel_stuck (subst_comp_cons c2 v1) r ->
+  eval_rel_stuck (comp_let c1 c2) r.
+Proof.
+  intros H. dependent induction H.
+  - intros. specialize (IHeval_rel_stuck c2 v1 r eq_refl H1).
+    econstructor. eapply step_let1; eauto. auto.
+  - intros. eapply step_let2 with (c2 := c2) in H. econstructor; eauto.
+Qed.
+
+Lemma eval_rel_stuck_let2 t1 t2 MR (c1 c1' : comp t1 [] MR) (c2 : comp t2 [t1] MR) :
+  eval_rel_stuck c1 (inr c1') -> eval_rel_stuck (comp_let c1 c2) (inr (comp_let c1' c2)).
+Proof.
+  intros H. dependent induction H.
+  - econstructor. eapply step_let1; eauto. eauto.
+  - eapply eval_rel_stuck_stuck. econstructor. eauto.
+Qed.
+
+Lemma eval_rel_stuck_let3 t1 t2 MR (c1 : comp t1 [] MR) (c2 : comp t2 [t1] MR) v2 :
+  eval_rel_stuck (comp_let c1 c2) (inl v2) ->
+  exists v1, eval_rel_stuck c1 (inl v1) /\ eval_rel_stuck (subst_comp_cons c2 v1) (inl v2).
+Proof.
+  intros H. dependent induction H.
+  - eapply step_let5 in H as Hstep.
+    destruct Hstep as [[v [Hv Hc2]] | [c1' [Hc1'1 Hc1'2]]].
+    + subst. exists v. split. constructor; auto. unfold step. simp observe.
+    + subst. specialize (IHeval_rel_stuck _ c1' _ _ eq_refl eq_refl).
+      destruct IHeval_rel_stuck as [v1 [Hv11 Hv12]].
+      exists v1. split; auto. econstructor; eauto.
+  - unfold step in H. simp observe in H. 
+    destruct (SmallStepSeq.observe c1); try destruct b; try discriminate.
+Qed.
+
+Lemma eval_rel_stuck_let4 t1 t2 MR (c1 : comp t1 [] MR) (c2 : comp t2 [t1] MR) c' :
+  eval_rel_stuck (comp_let c1 c2) (inr c') ->
+  (exists c'', eval_rel_stuck c1 (inr c'')) \/ (exists v1, eval_rel_stuck c1 (inl v1) /\ eval_rel_stuck (subst_comp_cons c2 v1) (inr c')). 
+Proof.
+  intros H. dependent induction H.
+  - eapply step_let5 in H as Hstep.
+    destruct Hstep as [[v [Hv Hc2]] | [c1' [Hc1'1 Hc1'2]]].
+    + subst. right. exists v. split; auto. eapply eval_rel_stuck_val. unfold step.
+      simp observe. auto.
+    + subst. specialize (IHeval_rel_stuck _ _ _ _ eq_refl eq_refl).
+      destruct IHeval_rel_stuck as [[c'' Hc''] | [v1 [Hv11 Hv12]] ].
+      * left. exists c''. econstructor; eauto.
+      * right. exists v1. split; auto. econstructor; eauto.
+  - left. dependent destruction H. exists c1. eapply eval_rel_stuck_stuck; eauto.
+Qed.
+
+Lemma step_eval_context_exposed_call:
+  forall (t1 t2 : vtype) (R : call_frame) (MR1 MR2 : mfix_ctx) (c : call_syn t2 MR2)
+    (E : eval_context t1 (R :: MR1) (inr c) true), step_eval_context true (inr c) E = None.
+Proof.
+  intros t1 t2 R MR1 MR2 c E.
+  dependent induction E; simp step_eval_context. auto.
+  cbn. rewrite IHE; auto.
+Qed.
+
+Lemma step_mfix_eval_context t1 t2 R MR1 MR2 (r : bredex t2 MR2 + call_syn t2 MR2) b
+      (E : eval_context t1 (R :: MR1) r b) (bodies : mfix_bodies [] MR1 R R) c' :
+  step_eval_context b r E = Some c' ->
+  step_eval_context _ r (ev_mfix b R bodies E) = Some (comp_mfix R bodies c').
+Proof.
+  generalize dependent c'. dependent induction E; destruct r; simp step_eval_context;
+    intros; try discriminate.
+  - cbn in *. intros. injection H. intros. simp subst_eval_context.
+    simp subst_eval_context in H. injection H. intros. subst. auto.
+  - cbn in H. injection H. intros. subst. simp subst_eval_context.
+    cbn. auto.
+  - cbn in H. simp step_eval_context in H.
+    destruct (step_eval_context b (inr c0) E) eqn : HE; try discriminate.
+    injection H. intros. subst. eapply IHE with (bodies := bodies) in HE as HE1; eauto.
+    destruct b; simp step_eval_context.
+    + assert (step_eval_context true (inr c0) E = None).
+      eapply step_eval_context_exposed_call.
+      rewrite HE in H0. discriminate.
+    + cbn. rewrite HE. auto.
+  - simp subst_eval_context. injection H. intros. subst. auto.
+  - rewrite H. cbn. auto.
+  - cbn. simp subst_eval_context. simp subst_eval_context in H. injection H.
+    intros. subst. auto.
+  - cbn. rewrite H. auto.
+  - simp subst_eval_context. injection H. intros. subst. auto.
+  - cbn. rewrite H; auto.
+Qed.
+
 Lemma step_mfix t R MR (bodies : mfix_bodies [] MR R R) (c c' : comp t [] (R :: MR)) : 
   step_rel c c' ->
   step_rel (comp_mfix _ bodies c) (comp_mfix _ bodies c').
 Proof.
-  intros [?]. constructor. unfold step in *.
-  simp observe. destruct (SmallStepSeq.observe c0); try destruct b; try discriminate.
-  f_equal. destruct r; simp step_eval_context.
-  - cbn. f_equal. injection H. clear H. intros.
-    simp step_eval_context in H.
-    cbn in H. injection H. intros. subst; auto.
-  - injection H. clear H. intros. clear c c' c0. rename c'0 into c.
-    destruct b.
-    + simp step_eval_context. admit.
-    + simp step_eval_context. cbn. rewrite H. auto.
-    dependent induction E.
-    + simp step_eval_context in H. discriminate.
-    + simp step_eval_context in H. cbn in H.
-      destruct (step_eval_context b (inr c1) E) eqn : Heq.
-      * injection H. clear H. intros. subst.
-        eapply IHE with (bodies := bodies) in Heq; eauto.
-        destruct b.
-        -- simp step_eval_context in Heq. simp step_eval_context.
-           admit.
-    destruct b.
-    + simp step_eval_context. 
-      simp step_eval_context in H.
-      dependent destruction E.
-      * simp step_eval_context in H. discriminate.
-      * simp normalize_eval_context. simp step_eval_context in H.
-        cbn in H. specialize (IHE c1 MR R bodies).
+  intros. dependent destruction H. 
+  constructor.
+  unfold step in *. simp observe. destruct (SmallStepSeq.observe c); try destruct b;
+    try discriminate.
+  f_equal. injection H. intros.  eapply step_mfix_eval_context. auto.
+Qed.
 
-injection H. clear H. intros. dependent induction E.
-      * simp step_eval_context in H. discriminate.
-      * simp normalize_eval_context. simp step_eval_context in H.
-        cbn in H.
+Lemma step_mfix_ret t R MR (bodies : mfix_bodies [] MR R R) (c : comp t [] (R :: MR)) v :
+  step c = inr v ->
+  step_rel (comp_mfix R bodies c) (comp_ret v).
+Proof.
+  intros. constructor. unfold step in *. simp observe.
+  destruct (SmallStepSeq.observe c); try destruct b; try discriminate.
+  cbn. simp step_eval_context. cbn. simp subst_eval_context.
+  simp step_bredex. injection H. intros. subst. auto.
+Qed.
 
-      admit.
-    + injection H. intros. rewrite H0. auto.
+Lemma normalize_eval_context_callv (t1 t2 : vtype) R MR
+      (ca : call_syn t2 (R :: MR))
+      (E : eval_context t1 (R :: MR) (inr ca) true) :
+  normalize_eval_context ca E = (ca && E).
+Proof.
+  dependent induction E. simp normalize_eval_context. auto.
+  simp normalize_eval_context. erewrite IHE; eauto.
+Qed.
+
+Lemma step_focused_mfix_context_VarZ (t1 t2 t3 : vtype) R MR
+      (x : var (t2, t3) R) (v : closed_value t2) (bodies : mfix_bodies [] MR R R)
+      (E : eval_context t1 (R :: MR) (inr (SmallStepSeq.callv (VarZ (l := MR)) x v)) true) : 
+  step_eval_context _ _ (ev_mfix _ R bodies E) =
+    Some (comp_mfix R bodies (subst_eval_context E (subst_comp_cons (nth_body bodies x) v) )).
+Proof.
+  simp step_eval_context.
+  rewrite normalize_eval_context_callv.
+  cbn. simp var_eq_neq. simp var_eq_elim. auto.
+Qed.
+
+Lemma step_focused_mfix_context_neq_VarZ (t1 t2 t3 : vtype) R1 R2 MR
+      (xR : var R2 MR) (x : var (t2, t3) R2) (v : closed_value t2) 
+      (bodies : mfix_bodies [] MR R1 R1)
+      (E : eval_context t1 (R1 :: MR) (inr (SmallStepSeq.callv (VarS (b := R1) xR) x v)) true) : 
+  step_eval_context _ _ (ev_mfix _ _ bodies E) = Some (push_eval_context (inr (SmallStepSeq.callv 
+                                  (VarS xR) x v)) E (comp_mfix_map bodies)
+                      (comp_call xR x v)).
+Proof.
+  simp step_eval_context. rewrite normalize_eval_context_callv. simp var_eq_neq.
+  Transparent remove_var. cbn. Opaque remove_var. auto.
+Qed.
+
+Lemma stuck_call_observe t1 t2 MR (c : comp t1 [] MR) (ca : call_syn t2 MR)
+      (E : eval_context t1 MR (inr ca) true) :
+  stuck_call c ca E -> SmallStepSeq.observe c = inl (bec _ E).
+Proof.
+  intros Hstuck. dependent induction Hstuck.
+  - simp observe. rewrite IHHstuck. auto.
+  - simp observe. auto.
+Qed.
+
+Lemma stuck_call_step_VarZ t1 t2 t3 R MR (c : comp t1 [] (R :: MR)) bodies
+      (x : var (t2, t3) R) (v : closed_value t2) E :
+  stuck_call c (SmallStepSeq.callv VarZ x v) E ->
+  step_rel (comp_mfix R bodies c) 
+           (comp_mfix R bodies (subst_eval_context E (subst_comp_cons (nth_body bodies x) v)) ).
+Proof.
+  intros. constructor. unfold step. apply stuck_call_observe in H.
+  simp observe. rewrite H. rewrite step_focused_mfix_context_VarZ. auto.
+Qed.
+
+Lemma stuck_call_step_neq_VarZ t1 t2 t3 R1 R2 MR (c : comp t1 [] (R1 :: MR)) bodies
+      (xR : var R2 MR) (x : var (t2, t3) R2) (v : closed_value t2) E :
+  stuck_call c (SmallStepSeq.callv (VarS xR) x v) E ->
+  step_rel (comp_mfix R1 bodies c)
+           (push_eval_context _ E (comp_mfix_map bodies) (comp_call xR x v)).
+Proof.
+  intros. constructor. unfold step. apply stuck_call_observe in H.
+  simp observe. rewrite H. rewrite step_focused_mfix_context_neq_VarZ.
+  auto.
+Qed.
+
+Lemma eval_rel_stuck_stuck_call_step t1 R MR (c1 c2 : comp t1 [] (R :: MR)) c3 r bodies :
+  eval_rel_stuck c1 (inr c2) ->
+  step_rel (comp_mfix R bodies c2) c3 ->
+  eval_rel_stuck c3 r ->
+  eval_rel_stuck (comp_mfix R bodies c1) r.
+Proof.
+  intros Hstuck. dependent induction Hstuck.
+  - intros. econstructor. eapply step_mfix; eauto. eapply IHHstuck; eauto.
+  - intros. econstructor; eauto.
+Qed.
+
+Lemma eval_rel_stuck_mfix_stuck_call_VarZ t1 t2 t3 R MR (c1 c2 : comp t1 [] (R :: MR)) r bodies
+      (x : var (t2, t3) R) (v : closed_value t2) E :
+  eval_rel_stuck c1 (inr c2) ->
+  stuck_call c2 (SmallStepSeq.callv VarZ x v) E ->
+  eval_rel_stuck 
+    (comp_mfix R bodies (subst_eval_context E (subst_comp_cons (nth_body bodies x) v))) r ->
+  eval_rel_stuck (comp_mfix R bodies c1) r.
+Proof.
+  intros. eapply eval_rel_stuck_stuck_call_step; eauto.
+  eapply stuck_call_step_VarZ. auto.
+Qed.
+
+Lemma eval_rel_stuck_mfix_stuck_call_neq_VarZ t1 t2 t3 R1 R2 MR (c1 c2 : comp t1 [] (R1 :: MR)) r bodies
+      (xR : var R2 MR) (x : var (t2, t3) R2) (v : closed_value t2) E :
+  eval_rel_stuck c1 (inr c2) ->
+  stuck_call c2 (SmallStepSeq.callv (VarS xR) x v) E ->
+  eval_rel_stuck (push_eval_context _ E (comp_mfix_map bodies) (comp_call xR x v)) r ->
+  eval_rel_stuck (comp_mfix R1 bodies c1) r.
+Proof.
+  intros. eapply eval_rel_stuck_stuck_call_step; eauto.
+  eapply stuck_call_step_neq_VarZ. auto.
+Qed.
+
+
+Lemma eval_rel_stuck_mfix_ret t R MR (c : comp t [] (R :: MR)) bodies v :
+  eval_rel_stuck c (inl v) ->
+  eval_rel_stuck (comp_mfix R bodies c) (inl v).
+Proof.
+  intros Heval. dependent induction Heval.
+  - econstructor. eapply step_mfix; eauto. eapply IHHeval; eauto.
+  - econstructor. eapply step_mfix_ret; eauto. apply eval_rel_stuck_val.
+    unfold step. simp observe. auto.
+Qed.
+
+(*
+Scheme Equality for vtype.
+*)
+(*
+#[local] Instance dec_eq_vtype : EqDec vtype.
+Proof.
+  red. intros x. induction x.
+  - intros y. destruct y; auto; right; intro; discriminate.
+  - intros y. destruct y; auto; try (right; intro; discriminate).
+    specialize (IHx y). destruct IHx; subst; auto. right. intro.
+    injection H. auto.
+  - admit.
+  - intros y. destruct y; auto; try (right; intro; discriminate).
+    specialize (IHx1 y1). specialize (IHx2 y2).
+    destruct IHx1; destruct IHx2; subst; auto.
+#[local] Instance uip_mfix_ctx : UIP mfix_ctx.
+Proof.
+  apply eqdec_uip. constructor.
 Admitted.
+*)
+
+(* either need to develop the mutually recursive eqdec instance on vtype/mfix_ctx
+
+*)
+(*
+Inductive push_eval_context_context : forall {t1 t2 MR1 MR2} (r : bredex t2 MR1 + call_syn t2 MR1)
+          (E : eval_context t1 MR1 r true)
+          (f : forall t Γ, comp t Γ MR1 -> comp t Γ MR2)
+          (E' : eval_context t2 MR2 r true), eval_context t1 MR2 r true -> Prop := 
+| pecc_hole t1 MR1 r (E : eval_context t1 MR1 r true) f  :
+  @push_eval_context_context t1 t1 MR1 MR1 r ev_hole f E E
+| pecc_let t1 t2 t3 MR1 MR2 r E1 c2 f E' E1' :
+  @push_eval_context_context t1 t3 MR1 MR2 r E1 f E' E1' ->
+  push_eval_context_context (t1 := t2) r (ev_let E1 c2) f E' (ev_let E1' (f _ [_] c2))
+
+.
+
+Lemma push_eval_context_context_ex : forall t1 t2 MR1 MR2 (r : bredex t2 MR1 + call_syn t2 MR1)
+          (E : eval_context t1 MR1 r true)
+          (f : forall t Γ, comp t Γ MR1 -> comp t Γ MR2)
+          (E' : eval_context t2 MR2 r true),
+    exists E'', @push_eval_context_context t1 t2 MR1 MR2 r E f E' E''.
+Proof.
+  intros t1 t2 MR1 MR2 r E. dependent induction E.
+  - intros. exists E'. eapply pecc_hole. econstructor. *)
+(*
+Equations push_eval_context_context {t1 t2 MR1 MR2} (r : bredex t2 MR1 + call_syn t2 MR1)
+          (E : eval_context t1 MR1 r true)
+          (f : forall t Γ, comp t Γ MR1 -> comp t Γ MR2)
+          (E' : eval_context t2 MR2 r true) : eval_context t1 MR2 r true :=
+  push_eval_context_context r ev_hole f E' := E';
+  push_eval_context_context r (ev_let E1 c2) f E' := 
+    ev_let (push_eval_context_context r E1 f E') (f _ [_] c2).
+    comp_let (push_eval_context r E1 f c) (f _ [_] c2).
+*)
+
+
+(* need to figure *)
+(*
+  what if I just relate this to observe in some way
+
+  stuck_call c ca E -> ...
+
+*)
