theories/AlmostStlc/ApproxCompTerm.v
@@ -1,0 +1,377 @@
+Require Export TypedVar.
+Require Export SyntaxSeq.
+Require Export SmallStepSeq.
+Require Export DenotationFacts.
+Require Export DenotationSeq.
+Require Export TypesEquiv.
+Require Export MapEFacts.
+Import List.ListNotations.
+Open Scope list_scope.
+From Equations Require Import Equations Signature.
+Require Import Coq.Program.Equality.
+Require Import ExtLib.Structures.Monad.
+Require Import Coq.Relations.Relation_Operators.
+Import MonadNotation.
+Local Open Scope monad_scope.
+Require Export SemanticsFactsSeq.
+Require Export CallMrecFacts.
+Require Export SemanticsFactsSeq2.
+Require Export SmallStepSeqFacts.
+Require Import Lia.
+Require Import Coq.Classes.Morphisms.
+Require Export ClosingSubst.
+Require Export LogicalApprox.
+Require Export SubstCommute.
+
+
+
+Inductive approx_comp_term {t MR} : forall (n : nat) (c1 c2 : comp t [] MR), Prop :=
+  approx_comp_term_intro n c1 c2 : 
+    (forall v1, eval_rel_stuck c1 (inl v1) -> eval_rel_stuck c2 (inl v1)) /\
+    (forall tin tout Rcall (xR : var Rcall MR) (x : var (tin, tout) Rcall) 
+         (vcall : closed_value tin) (E1 :eval_context t MR (inr (SmallStepSeq.callv xR x vcall) ) true) 
+         (c1' : comp t [] MR),
+  eval_rel_stuck c1 (inr c1') -> stuck_call c1' (SmallStepSeq.callv xR x vcall) E1 ->
+  exists c2' E2, eval_rel_stuck c2 (inr c2') /\ stuck_call c2' (SmallStepSeq.callv xR x vcall) E2 /\
+           forall vout n', n' < n -> approx_comp_term n' (subst_eval_context E1 vout) (subst_eval_context E2 vout)) -> approx_comp_term n c1 c2.
+
+(*
+Inductive approx_comp_term {t MR} : forall (c1 c2 : comp t [] MR), Prop :=
+  approx_comp_term_intro c1 c2 : 
+    (forall v1, eval_rel_stuck c1 (inl v1) -> eval_rel_stuck c2 (inl v1)) /\
+    (forall tin tout Rcall (xR : var Rcall MR) (x : var (tin, tout) Rcall) 
+         (vcall : closed_value tin) (E1 :eval_context t MR (inr (SmallStepSeq.callv xR x vcall) ) true) 
+         (c1' : comp t [] MR),
+  eval_rel_stuck c1 (inr c1') -> stuck_call c1' (SmallStepSeq.callv xR x vcall) E1 ->
+  exists c2' E2, eval_rel_stuck c2 (inr c2') /\ stuck_call c2' (SmallStepSeq.callv xR x vcall) E2 /\
+           forall vout, approx_comp_term (subst_eval_context E1 vout) (subst_eval_context E2 vout)) -> approx_comp_term c1 c2.
+*)
+
+Lemma approx_comp_approx_comp_term n t MR m (c1 c2 : comp t [] MR) :
+  approx_comp_term n c1 c2 -> approx_comp n approx_val m c1 -> approx_comp n approx_val m  c2.
+Proof.
+  generalize dependent t. revert MR. 
+  induction n as [ n IHn ] using (well_founded_induction lt_wf).
+  intros MR t m c1 c2 Hc12 Hmc1.
+  constructor. intros j Hj. inversion Hmc1. subst.
+  specialize (H j Hj) as [Hret Hstuck].
+  split.
+  - intros. specialize (Hret _ H) as [v [Hv11 Hv12]]. clear Hstuck.
+    exists v. inversion Hc12. subst. destruct H0 as [Hret _]. split; auto.
+  - intros. specialize (Hstuck _ _ _ _ _ _ _ H).
+    destruct Hstuck as [vcall [E [c' [HE1 [HE2 [HE3 HE4]]]]]].
+    inversion Hc12. subst. destruct H0 as [_ Hstuck].
+    eapply Hstuck in HE2; eauto. destruct HE2 as [c'' [E' [HE'1 [HE'2 HE'3]]]].
+    exists vcall, E', c''. split; auto. split; auto. split; auto.
+    intros. specialize (HE4 j'' vvret vret H0 H1).
+    eapply IHn; eauto. lia. eapply HE'3. lia.
+Qed.
+
+Lemma approx_comp_term_refl n t MR (c : comp t [] MR) : 
+  approx_comp_term n c c.
+Proof.
+  generalize dependent t. revert MR.
+  induction n as [ n IHn ] using (well_founded_induction lt_wf).
+  intros.
+  constructor. split.
+  auto. intros. eexists. eexists. split; eauto.
+Qed.
+
+
+Lemma approx_comp_term_trans n : forall t MR (c1 c2 c3 : comp t [] MR),
+    approx_comp_term n c1 c2 -> approx_comp_term n c2 c3 ->
+    approx_comp_term n c1 c3.
+Proof.
+  induction n as [n IHn] using (well_founded_induction lt_wf).
+  intros. inversion H. subst. inversion H0. subst. clear H0 H.
+  constructor. split.
+  - destruct H1 as [Hret12 _]. destruct H2 as [Hret23 _].
+    intros. eapply Hret12 in H. auto.
+  - destruct H1 as [_ Hstuck12]. destruct H2 as [_ Hstuck23].
+    intros. eapply Hstuck12 in H as H1; eauto. 
+    destruct H1 as [c2' [E2 [H1 [H2 H3]]]].
+    eapply Hstuck23 in H1 as H4; try apply H2.
+    destruct H4 as [c3' [E3 [HE31 [HE32 HE33]]]].
+    exists c3'. exists E3.
+    split; [ | split]; eauto.
+Qed.
+
+Lemma approx_comp_term_step1 n t MR (c1 c2 : comp t [] MR) :
+  step_rel c1 c2 -> approx_comp_term n c1 c2.
+Proof.
+  intros.
+  constructor. split.
+  - intros. dependent destruction H0.
+    + enough (c2 = c0). subst. auto. dependent destruction H.
+      dependent destruction H0. rewrite H in H0. injection H0. auto.
+    + dependent destruction H. rewrite H in H0. discriminate.
+  - intros. exists c1', E1. split; [ | split]; eauto.
+    + dependent destruction H0.
+      * enough (c2 = c0). subst. auto. dependent destruction H.
+        dependent destruction H0. rewrite H in H0. injection H0. auto.
+      * dependent destruction H. eapply stuck_call_stuck' in H0.
+        rewrite H in H0. discriminate.
+    + intros. apply approx_comp_term_refl.
+Qed.
+
+Lemma approx_comp_term_step2 n t MR (c1 c2 : comp t [] MR) :
+  step_rel c1 c2 -> approx_comp_term n c2 c1.
+Proof.
+  intros. constructor. split.
+  - intros. econstructor; eauto.
+  - intros. exists c1', E1. split; [ | split]; eauto.
+    econstructor; eauto. intros. apply approx_comp_term_refl.
+Qed.
+
+       
+Lemma approx_comp_term_comp_call n t1 MR t2 (cbody : comp t2 [t1] MR) (varg : value t1 []) :
+  approx_comp_term n (subst_comp_cons cbody varg) (comp_app (val_abs cbody) varg).
+Proof.
+  apply approx_comp_term_step2. constructor. unfold step.
+  simp observe. cbn. simp step_eval_context. simp subst_eval_context.
+  auto.
+Qed.
+
+Lemma lower_approx_comp_term n : forall n' t MR (c1 c2 : comp t [] MR),
+    n' < n -> approx_comp_term n c1 c2 -> approx_comp_term n' c1 c2.
+Proof.
+  induction n as [n IHn] using (well_founded_induction lt_wf).
+  intros. inversion H0. subst. destruct H1 as [Hret Hstuck].
+  constructor. split; auto.
+  intros. eapply Hstuck in H1; eauto. destruct H1 as [c2' [E2 [? [? ?]]]].
+  eexists. eexists. split; [ | split]; eauto.
+Qed.
+
+Lemma approx_comp_term_let_cong n : forall t1 t2 MR 
+       (c1 c1' : comp t1 [] MR) (c2 c2' : comp t2 [t1] MR),
+    approx_comp_term n c1 c1' -> (forall v, approx_comp_term n (subst_comp_cons c2 v) (subst_comp_cons c2' v)) ->
+    approx_comp_term n (comp_let c1 c2) (comp_let c1' c2').
+Proof.
+  induction n as [n IHn] using (well_founded_induction lt_wf).
+  intros. inversion H. subst. constructor. split; intros.
+  - eapply eval_rel_stuck_let3 in H2. rename v1 into v2. destruct H2 as [v1 [Hv11 Hv12]].
+    destruct H1 as [Hret1 _].
+    eapply eval_rel_stuck_let1; eauto.
+    specialize (H0 v1). inversion H0. subst. destruct H1 as [Hret2 _].
+    auto.
+  - eapply eval_rel_stuck_let4 in H2 as H2'.
+    destruct H2' as [[c' Hc'] | [v1 [Hv11 Hv12]] ].
+    + eapply eval_rel_stuck_let2 with (c2 := c2) in Hc' as Hc''.
+      eapply eval_rel_stuck_inj in Hc'' as Heq; try apply H2. subst.
+      inversion H. subst. destruct H4 as [Hret1 Hstuck1].
+      dependent destruction H3.
+      eapply Hstuck1 in Hc' as Hc'''; eauto.
+      destruct Hc''' as [c'' [E2 [? [? ?]]]].
+      eapply eval_rel_stuck_let2 with (c2 := c2') in H4 as ?.
+      eexists. eexists.
+      split; [ | split]; eauto. constructor. eauto.
+      intros. simp subst_eval_context.
+      eapply IHn; eauto. intros. eapply lower_approx_comp_term; eauto.
+    + destruct H1 as [Hret1 Hstuck1]. eapply Hret1 in Hv11 as Hv13.
+      specialize (H0 v1). inversion H0. subst.
+      destruct H1 as [Hret2 Hstuck2]. eapply Hstuck2 in Hv12 as ?; eauto.
+      destruct H1 as [c2'' [E2 [? [? ?]]]]. exists c2'', E2. split; [ | split]; auto.
+      eapply eval_rel_stuck_let1; eauto.
+Qed.
+    
+Lemma approx_comp_term_let_ret_r n t MR (c : comp t [] MR) :
+  approx_comp_term n c (comp_let c (comp_ret (val_var VarZ))).
+Proof.
+  generalize dependent t. revert MR.
+  induction n as [n IHn] using (well_founded_induction lt_wf).
+  intros.
+  constructor. split.
+  - intros. eapply eval_rel_stuck_let1; eauto.
+    unfold subst_comp_cons. simp subst_comp. simp subst_var.
+    apply eval_rel_stuck_val. unfold step. simp observe. auto.
+  - intros. exists (comp_let c1' (comp_ret (val_var VarZ))), (ev_let E1 (comp_ret (val_var VarZ))).
+    split; [ | split].
+    + apply eval_rel_stuck_let2; auto.
+    + constructor. auto.
+    + intros. rewrite subst_eval_context_equation_2. 
+      apply IHn. auto.
+Qed.
+
+Lemma approx_comp_term_let_ret_r' n t MR (c : comp t [] MR) :
+  approx_comp_term n (comp_let c (comp_ret (val_var VarZ))) c.
+Proof.
+  generalize dependent t. revert MR.
+  induction n as [n IHn] using (well_founded_induction lt_wf).
+  intros. constructor. split.
+  - intros. eapply eval_rel_stuck_let3 in H. destruct H as [v1' [Hv1'1 Hv1'2]].
+    unfold subst_comp_cons in Hv1'2. simp subst_comp in Hv1'2.
+    simp subst_var in Hv1'2. dependent destruction Hv1'2; auto.
+    exfalso. dependent destruction H.
+  - intros. eapply eval_rel_stuck_let4 in H as H'.
+    destruct H' as [[c' Hc'] | [v1' [Hv1'1 Hv1'2]]].
+    + eapply eval_rel_stuck_let2 in Hc' as Hc''. 
+      eapply eval_rel_stuck_inj in H; try eapply Hc''. subst.
+      dependent destruction H0.
+      eexists. eexists. split; [ | split]; eauto.
+      intros. simp subst_eval_context.
+    + unfold subst_comp_cons in Hv1'2. simp subst_comp in Hv1'2.
+      simp subst_var in Hv1'2. dependent destruction Hv1'2;
+      dependent destruction H1.
+Qed.
+
+Lemma approx_comp_term_let_assoc n : forall t1 t2 t3 MR 
+      (c1 : comp t1 [] MR) (c2 : comp t2 [t1] MR) (c3 : comp t3 [t2] MR),
+  approx_comp_term n 
+                   (comp_let (comp_let c1 c2) c3) 
+                   (comp_let c1 (comp_let c2 (weaken_r_comp _ c3))).
+Proof.
+  induction n as [n IHn] using (well_founded_induction lt_wf). 
+  intros. constructor. split.
+  - intros. rename v1 into v3. eapply eval_rel_stuck_let3 in H as H12.
+    destruct H12 as [v2 [Hv21 Hv22]].
+    eapply eval_rel_stuck_let3 in Hv21 as H1.
+    destruct H1 as [v1 [Hv11 Hv12]].
+    eapply eval_rel_stuck_let1; eauto. unfold subst_comp_cons.
+    simp subst_comp. eapply eval_rel_stuck_let1; eauto.
+    clear - Hv22. rewrite subst_comp_weaken_r. auto.
+  - intros. rename c1' into cf'. rename E1 into Ef.
+    eapply eval_rel_stuck_let4 in H as H'. 
+    destruct H' as [ [c12 Hc12] | [v2 [Hv21 Hv22]] ].
+    + eapply eval_rel_stuck_let4 in Hc12 as H'.
+      destruct H' as [ [c1' Hc1'] | [v1 [Hv11 Hv12]] ].
+      * eapply eval_rel_stuck_ex_call in Hc1' as Hcall.
+        destruct Hcall as [t' [ca [E1 HE1]]].
+        eapply stuck_call_let with (c2 := c2) in HE1 as HE1'.
+        eapply stuck_call_let with (c2 := c3) in HE1'.
+        eapply eval_rel_stuck_let2 with (c2 := c2) in Hc1' as Hc1''.
+        eapply eval_rel_stuck_let2 with (c2 := c3) in Hc1''.
+        eapply eval_rel_stuck_inj in H; try apply Hc1''. subst.
+        eapply stuck_call_inj in H0; try apply HE1'; eauto. destruct H0 as [? [? ?]].
+        subst.
+        exists (comp_let c1' (comp_let c2 (weaken_r_comp [t2] c3))), (ev_let E1 (comp_let c2 (weaken_r_comp _ c3))). 
+        split; [ | split].
+        -- apply eval_rel_stuck_let2; auto.
+        -- constructor. auto.
+        -- intros. simp subst_eval_context.
+      * exists (comp_let c12 c3).
+        eapply eval_rel_stuck_ex_call in Hv12 as Hcall.
+        destruct Hcall as [t' [ca [E1 HE1]]]. 
+        eapply stuck_call_let with (c2 := c3) in HE1 as HE1'.
+        eapply eval_rel_stuck_let2 with (c2 := c3) in Hv12 as Hv12'; eauto.
+        assert (Hc123 : eval_rel_stuck (comp_let (comp_let c1 c2) c3) (inr (comp_let c12 c3))).
+        eapply eval_rel_stuck_let2. eapply eval_rel_stuck_let1; eauto.
+        eapply eval_rel_stuck_inj in Hc123 as Hc123';  try apply H. subst.
+        eapply stuck_call_inj in H0; eauto. destruct H0 as [? [? ?]]. subst.
+        exists (ev_let E1 c3).
+        split; [ | split].
+        -- eapply eval_rel_stuck_let1; eauto. unfold subst_comp_cons.
+           simp subst_comp. rewrite subst_comp_weaken_r. auto.
+        -- constructor. auto.
+        -- intros. apply approx_comp_term_refl.
+    + eapply eval_rel_stuck_let3 in Hv21 as H'. destruct H' as [v1 [Hv11 Hv12]].
+      exists cf', Ef. split; [ | split].
+      * eapply eval_rel_stuck_let1; eauto. unfold subst_comp_cons.
+        simp subst_comp. rewrite subst_comp_weaken_r. auto.
+        eapply eval_rel_stuck_let1; eauto.
+      * auto.
+      * intros. apply approx_comp_term_refl.
+Qed.
+
+Lemma approx_comp_term_let_assoc' n : forall t1 t2 t3 MR 
+      (c1 : comp t1 [] MR) (c2 : comp t2 [t1] MR) (c3 : comp t3 [t2] MR),
+  approx_comp_term n 
+                   (comp_let c1 (comp_let c2 (weaken_r_comp _ c3)))
+                   (comp_let (comp_let c1 c2) c3).
+Proof.
+  induction n as [n IHn] using (well_founded_induction lt_wf). 
+  intros. constructor. split.
+  - intros. rename v1 into v3. eapply eval_rel_stuck_let3 in H as H12.
+    destruct H12 as [v2 [Hv21 Hv22]].
+    unfold subst_comp_cons in Hv22. simp subst_comp in Hv22.
+    rewrite subst_comp_weaken_r in Hv22.
+    eapply eval_rel_stuck_let3 in Hv22 as H'.
+    destruct H' as [v3' [Hv31 Hv32] ].
+    eapply eval_rel_stuck_let1; eauto. eapply eval_rel_stuck_let1; eauto.
+  - intros. rename c1' into cf'. rename E1 into Ef.
+    eapply eval_rel_stuck_let4 in H as H'. 
+    destruct H' as [ [c1' Hc1'] | [v1 [Hv11 Hv12]] ].
+    + eapply eval_rel_stuck_let2 with (c2 := (comp_let c2 (weaken_r_comp [t2] c3))) in Hc1' as Hc1''.
+      eapply eval_rel_stuck_inj in H as ?; try apply Hc1''; subst.
+      eapply eval_rel_stuck_let2 with (c2 := c2) in Hc1' as Hc1'''.
+      eapply eval_rel_stuck_let2 with (c2 := c3) in Hc1'''.
+      eapply eval_rel_stuck_ex_call in Hc1' as Hcall.
+      destruct Hcall as [t' [ca [E1 HE1]]].
+      eapply stuck_call_let with (c2 := (comp_let c2 (weaken_r_comp [t2] c3))) in HE1 as HE1'.
+      eapply stuck_call_inj in HE1' as ?; try apply H0. destruct H1 as [? [? ?]]; subst. 
+      exists (comp_let (comp_let c1' c2) c3). eexists.
+      split; auto. split. econstructor. econstructor. eauto.
+      intros. simp subst_eval_context.
+    + unfold subst_comp_cons in Hv12. simp subst_comp in Hv12.
+      rewrite subst_comp_weaken_r in Hv12.
+      eapply eval_rel_stuck_let4 in Hv12 as H'.
+      destruct H' as [ [c2' Hc2']  | [v2 [Hv21 Hv22]]].
+      * eapply eval_rel_stuck_let2 with (c2 := c3) in Hc2' as Hc2''.
+        eapply eval_rel_stuck_inj in Hv12 as ?; try apply Hc2''; subst.
+        dependent destruction H0. eexists. eexists.
+        split; [ | split].
+        -- eapply eval_rel_stuck_let2. eapply eval_rel_stuck_let1; eauto.
+        -- econstructor. eauto.
+        -- intros. simp subst_eval_context. eapply approx_comp_term_refl.
+      * exists cf', Ef. split; [ | split].
+        -- eapply eval_rel_stuck_let1; eauto. eapply eval_rel_stuck_let1; eauto.  
+        -- auto.
+        -- intros. apply approx_comp_term_refl.
+Qed.
+
+Lemma  approx_comp_term_mfix_ret:
+  forall (t : vtype) (MR : mfix_ctx) (R1 : call_frame)
+    (bodies : mfix_bodies [] MR R1 R1) (vvret : value t []) 
+    (n : nat),
+    approx_comp_term n (comp_mfix R1 bodies (comp_ret vvret)) (comp_ret vvret).
+Proof.
+  intros t MR R1 bodies vvret n.
+  constructor. split.
+  - intros. constructor. unfold step. simp observe.
+    dependent destruction H.
+    dependent destruction H. simp subst_eval_context in H0.
+    simp step_brex in H0. dependent destruction H0; auto.
+    dependent destruction H.
+  - intros. dependent destruction H.
+    + dependent destruction H. simp subst_eval_context in H0.
+      simp step_bredex in H0. dependent destruction H0. dependent destruction H.
+      dependent destruction H.
+    + dependent destruction H.
+Qed.
+
+Lemma approx_comp_term_mfix_let:
+  forall (t1 t2 t3 : vtype) (MR : mfix_ctx) (R1 : call_frame) (tin : vtype) (vcall : closed_value tin) 
+    (R2 : call_frame) (x : var (tin, t3) R2) (xR : var R2 MR)
+    (E : eval_context t1 (R1 :: MR) (inr (SmallStepSeq.callv (VarS (b := R1) xR) x vcall)) true) (c : comp t2 [t1] (R1 :: MR))
+    (bodies : mfix_bodies [] MR R1 R1) (E' : eval_context t1 MR (inr (SmallStepSeq.callv xR x vcall)) true) 
+    (vvret : value t3 []) (n : nat),
+    approx_comp_term n (comp_mfix R1 bodies (comp_let (subst_eval_context E (comp_ret vvret)) c))
+                     (comp_let (subst_eval_context E' (comp_ret vvret)) (comp_mfix R1 (weaken_r_bodies bodies) c)).
+Proof.
+  intros t1 t2 t3 MR R1 tin vcall R2 x xR E c bodies E' vvret n.
+Admitted.
+(* weird mismatch of *)
+Lemma stuck_call_push_eval_context_mfix:
+  forall (t : vtype) (R1 R2 : call_frame) (MR : mfix_ctx) (bodies : mfix_bodies [] MR R1 R1)
+    (tin tout : vtype) (x : var (tin, tout) R2) (xR : var R2 MR)
+    (vcall : closed_value tin)
+    (E : eval_context t (R1 :: MR) (inr (SmallStepSeq.callv (VarS (b := R1) xR) x vcall)) true),
+    exists E', 
+    stuck_call
+      (push_eval_context (inr (SmallStepSeq.callv (VarS xR) x vcall)) E (comp_mfix_map bodies)
+                         (comp_call xR x vcall)) 
+      (SmallStepSeq.callv xR x vcall)
+      E' /\
+      (forall vvret n, approx_comp_term n (comp_mfix R1 bodies (subst_eval_context E (comp_ret vvret)))  
+                  (subst_eval_context E' (comp_ret vvret))).
+Proof.
+  intros.
+  dependent induction E.
+  - simp push_eval_context. exists ev_hole. split. constructor. intros. simp subst_eval_context.
+    apply approx_comp_term_mfix_ret.
+  - simp push_eval_context. simp subst_eval_context_ctx.
+    specialize (IHE _ _ _ _ _ _ _ bodies _ eq_refl eq_refl JMeq_refl eq_refl JMeq_refl).
+    destruct IHE as [E' [HE'1 HE'2]]. econstructor. split. econstructor. eauto.
+    intros. simp subst_eval_context. unfold comp_mfix_map.
+    apply approx_comp_term_mfix_let.
+Qed.
+
